Weidenbach_Book/DPLL_W.thy
@@ -1,6 +1,6 @@
 theory DPLL_W
 imports
-  Entailment_Definition.Partial_Clausal_Logic
+  Entailment_Definition.Partial_Herbrand_Interpretation
   Entailment_Definition.Partial_Annotated_Clausal_Logic
   Weidenbach_Book_Base.Wellfounded_More
 begin
